{
 "cells": [
  {
   "cell_type": "markdown",
   "metadata": {},
   "source": [
    "**Name:** Alliah Mari O. Soro√±o\n",
    "\n",
    "**Program and Year:** BSCS - 1\n",
    "\n",
    "**Date Submitted:** May 14, 2024\n",
    "\n",
    "**Course and Description:** CIS 1203 - Discrete Structures\n",
    "\n",
    "**Lecture:** 1"
   ]
  },
  {
   "cell_type": "markdown",
   "metadata": {},
   "source": [
    "****\n",
    "### $\\textbf{Problem 1:}$\n",
    "\n",
    "<b><u>Problem</u></b>\n",
    "\n",
    "Recall the definition of a rational number, denoted as $\\mathbb{Q}$. \n",
    "\n",
    "Prove that the Euler's number $e = \\Sigma_{k=0}^\\infty \\frac{1}{k!} \\notin \\mathbb{Q}$. A factorial is defined as $k! = (k)(k-1)(k-2)(k-3)..., \\forall k \\in \\mathbb{Z}^+$, note that $0! = 1$. Furthermore, a sum notation $\\Sigma_{k=0}^\\infty k = 0+ 1 + 2 + 3 +....+...$\n",
    "\n",
    "<b><u>Solution</u></b>\n",
    "\n",
    "<b> Step 1:</b>\n",
    "\n",
    "To demonstrate that Euler's number $e$ is irrational, we'll use a proof by contradiction.\n",
    "Assume, for the sake of argument, that $e$  is rational.\n",
    "This implies that e can be written as a fraction of two integers, say $p$ and $q$, where $q \\neq 0$.\n",
    "\n",
    "Therefore, we know that:\n",
    "\n",
    "\n",
    "- $e = \\frac{p}{q}$\n",
    "\n",
    "<b> Step 2: </b> \n",
    "\n",
    "Now, we must remember the definition of $e$ as the sum of the series $\\sum_{k=0}^\\infty \\frac{1}{k!}$. This means that:\n",
    "\n",
    "\n",
    "- $ e = \\frac{1}{0!} + \\frac{1}{1!} + \\frac{1}{2!} + \\frac{1}{3!} + \\ldots $\n",
    "\n",
    "<b> Step 3: </b> \n",
    "\n",
    "For this step, consider the partial sum of the series:\n",
    "\n",
    "- $ S_n = \\frac{1}{0!} + \\frac{1}{1!} + \\frac{1}{2!} + \\frac{1}{3!} + \\ldots + \\frac{1}{n!} $\n",
    "\n",
    "For some positive integer $n$. Since each term in the series is positive, $S_n$ is increasing and bounded above by $e$, thus $S_n$ converges to $e$ as $n$ approaches infinity.\n",
    "\n",
    "<b> Step 4: </b> \n",
    "\n",
    "Afterwards, consider the number: \n",
    "- $ q! \\cdot S_n = q! \\cdot \\left(\\frac{1}{0!} + \\frac{1}{1!} + \\frac{1}{2!} + \\frac{1}{3!} + \\ldots + \\frac{1}{n!}\\right) $\n",
    "\n",
    "<b> Step 5: </b> \n",
    "\n",
    "Expanding this equation would result to:\n",
    "- $ q! \\cdot S_n = q! + \\frac{q!}{1!} + \\frac{q!}{2!} + \\frac{q!}{3!} + \\ldots + \\frac{q!}{n!} $\n",
    "\n",
    "<b> Step 6: </b>\n",
    "\n",
    "Every term in this expression is an integer.  Since $S_n$ converges to $e$, $q! \\cdot S_n$ should be very close to $q! \\cdot e = p$. This implies that $p - q! \\cdot S_n$ should be a very small positive integer.\n",
    "\n",
    "- $ p - q! \\cdot S_n = p - (q! + \\frac{q!}{1!} + \\frac{q!}{2!} + \\frac{q!}{3!} + \\ldots + \\frac{q!}{n!}) $\n",
    "\n",
    "- $ p - q! \\cdot S_n = p - q! - \\frac{q!}{1!} - \\frac{q!}{2!} - \\frac{q!}{3!} - \\ldots - \\frac{q!}{n!} $\n",
    "\n",
    "- $ p - q! \\cdot S_n = (p - q!) - \\frac{q!}{1!} - \\frac{q!}{2!} - \\frac{q!}{3!} - \\ldots - \\frac{q!}{n!} $\n",
    "\n",
    "<b> Step 7: </b>\n",
    "\n",
    "Each number in the parenthesis is an integer, and each term in the summation is a fraction with the denominator greater than 1. Therefore, $p - q! \\cdot S_n$ must be a non-zero positive integer. \n",
    "\n",
    "Nonetheless this conflicts with our assumption that $e = \\frac{p}{q}$ because $q! \\cdot S_n$ should be very close to $p$ but is not exactly equal to it, leading to a contradiction. \n",
    "\n",
    "**Therefore, our assumption that $e$ is rational must be false, and thus $e$ is irrational.**\n",
    "\n",
    "\n",
    "****\n",
    "\n"
   ]
  },
  {
   "cell_type": "markdown",
   "metadata": {},
   "source": [
    "### $\\textbf{Problem 2:}$\n",
    "\n",
    "<b><u>Problem</u></b>\n",
    "\n",
    "Prove Minkowski's Inequality for sums, $\\forall \\ p>1, (a_k, b_k)>0$:\n",
    "\\begin{gather}\n",
    "\\begin{bmatrix}\n",
    "\\Sigma_{k=1}^n |a_k + b_k|^p\n",
    "\\end{bmatrix}^\\frac{1}{p}\n",
    "\\leq\n",
    "\\begin{bmatrix}\n",
    "\\Sigma_{k=1}^n |a_k|^p\n",
    "\\end{bmatrix}^\\frac{1}{p}\n",
    "+\n",
    "\\begin{bmatrix}\n",
    "\\Sigma_{k=1}^n |b_k|^p\n",
    "\\end{bmatrix}^\\frac{1}{p}\n",
    "\\end{gather}\n",
    "\n",
    "<b><u>Solution</u></b>\n",
    "\n",
    "<b>Step 1: </b>\n",
    "\n",
    "Begin with using the  Holder's inequality:\n",
    "- $\\sum_{k=1}^{n} |a_k b_k| \\leq \\left( \\sum_{k=1}^{n} |a_k|^p \\right)^{\\frac{1}{p}} \\left( \\sum_{k=1}^{n} |b_k|^q \\right)^{\\frac{1}{q}}$\n",
    "\n",
    "<b>Step 2: </b> \n",
    "\n",
    "Define: \n",
    "- $a_k = |x_k|^p $ , $ b_k = |y_k|^p $\n",
    "\n",
    "<b>Step 3: </b>\n",
    "\n",
    "Using Holder's inequality, apply it with its definition (Defined through the previous step):\n",
    "- $ \\sum_{k=1}^{n} |x_k y_k|^p \\leq \\left( \\sum_{k=1}^{n} |x_k|^p \\right)^{\\frac{1}{p}} \\left( \\sum_{k=1}^{n} |y_k|^q \\right)^{\\frac{1}{q}} $\n",
    "\n",
    "<b>Step 4: </b> \n",
    "\n",
    "Take the $p$-th root of both sides:\n",
    "- $ \\left( \\sum_{k=1}^{n} |x_k y_k|^p \\right)^{\\frac{1}{p}} \\leq \\left( \\sum_{k=1}^{n} |x_k|^p \\right)^{\\frac{1}{p}} \\left( \\sum_{k=1}^{n} |y_k|^p \\right)^{\\frac{1}{q}} \\ $\n",
    "\n",
    "<b>Step 5: </b> \n",
    "\n",
    "Use the relationship between $p$ and $q$:\n",
    "- $ \\left( \\sum_{k=1}^{n} |x_k y_k|^p \\right)^{\\frac{1}{p}} \\leq \\left( \\sum_{k=1}^{n} |x_k|^p \\right)^{\\frac{1}{p}} \\left( \\sum_{k=1}^{n} |y_k|^p \\right)^{\\frac{p-1}{p}} \\ $\n",
    "\n",
    "<b>Step 6: </b> \n",
    "\n",
    "Recognize that: \n",
    "- $ \\frac{p-1}{p} = 1 - \\frac{1}{p} \\ $\n",
    "\n",
    "<b>Step 7: </b> \n",
    "\n",
    "Apply Holder's inequality to remove the $ \\frac{p-1}{p}\\ $ term:\n",
    "- $ \\left( \\sum_{k=1}^{n} |y_k|^p \\right)^{\\frac{p-1}{p}} \\leq n^{\\frac{p-1}{p}} \\left( \\sum_{k=1}^{n} |y_k|^p \\right)^{\\frac{1}{p}} \\ $\n",
    "\n",
    "<b>Step 8: </b> \n",
    "\n",
    "Substitute this equation from the previous step back into the inequality:\n",
    "- $ \\left( \\sum_{k=1}^{n} |x_k + y_k|^p \\right)^{\\frac{1}{p}} \\leq n^{\\frac{1}{p}} \\left( \\sum_{k=1}^{n} |x_k|^p \\right)^{\\frac{1}{p}} \\left( \\sum_{k=1}^{n} |y_k|^p \\right)^{\\frac{1}{p}} \\ $\n",
    "\n",
    "<b>Step 9: </b> \n",
    "\n",
    "Acknowledge that the obtained expression as its final form:\n",
    "- $ \\left( \\sum_{k=1}^{n} |x_k + y_k|^p \\right)^{\\frac{1}{p}} \\leq n^{\\frac{1}{p}} \\left( \\sum_{k=1}^{n} |x_k|^p \\right)^{\\frac{1}{p}} \\left( \\sum_{k=1}^{n} |y_k|^p \\right)^{\\frac{1}{p}} \\ $\n",
    "\n",
    "<br>\n",
    "\n",
    "**Therefore, we conclude that  Minkowski's inequality for sums is used.**\n",
    "\n",
    "\n",
    "****\n"
   ]
  },
  {
   "cell_type": "markdown",
   "metadata": {},
   "source": [
    "### $\\textbf{Problem 3:}$\n",
    "\n",
    "<b><u>Problem</u></b>\n",
    "\n",
    "Prove the triangle inequality $|x+y| \\leq |x| + |y|, \\forall (x,y) \\in \\mathbb{R}$\n",
    "\n",
    "<b><u>Solution</u></b>\n",
    "\n",
    "<b>Step 1: </b> \n",
    "\n",
    "Define the absolute value\n",
    "- Definition:\n",
    "\\begin{gathered}\n",
    "{|x| = }\n",
    "\\begin{cases}\n",
    "x,&{x \\geq 0}\\\\ -x,&{x < 0}\n",
    "\\end{cases}\n",
    "\\end{gathered}\n",
    "\n",
    "- Hence, we must solve for 4 cases to prove this point:\n",
    "\n",
    "\\begin{gathered}\n",
    "\\textbf{Case 1: }{x \\geq 0, y \\geq 0} \\\\\n",
    "\\textbf{Case 2: }{x < 0, y < 0} \\\\\n",
    "\\textbf{Case 3: }{x \\geq 0, y < 0} \\\\\n",
    "\\textbf{Case 4: }{x < 0, y \\geq 0} \\\\\n",
    "\\end{gathered}\n",
    "\n",
    "$ \\textbf{Case 1:} $ $x \\geq 0, y \\geq 0$\n",
    "\n",
    "- Let, $|x + y| = x + y$, and $|x| = x, |y| = y$\n",
    "- Substitution:\n",
    "\\begin{gathered}\n",
    "|x + y| = x + y = |x| + |y|\n",
    "\\end{gathered}\n",
    "\n",
    "$ \\textbf{Case 2:} $ $x < 0, y < 0$\n",
    "\n",
    "- Let, $|x + y| = -(x + y)$, and $|x| = -x, |y| = -y$\n",
    "- Substitution:\n",
    "\\begin{gathered}\n",
    "|x + y| = -(x + y) = -x + (-y) = |x| + |y|\n",
    "\\end{gathered}\n",
    "\n",
    "$ \\textbf{Case 3:} $ $x \\geq 0, y < 0$\n",
    "\n",
    "- Let, $|x| = x, |y| = -y$\n",
    "- Substitution:\n",
    "\\begin{gathered}\n",
    "|x + y| \\leq x - y\n",
    "\\end{gathered}\n",
    "- Since, $x$ and $y$ are different signs, let's consider two sub-cases for $|x + y|$:\n",
    "\\begin{gathered}\n",
    "x + y, x + y \\geq 0 \\\\\n",
    "-(x + y), x + y < 0 \\\\\n",
    "\\end{gathered}\n",
    "\n",
    "For $x + y \\geq 0$:\n",
    "\\begin{gathered}\n",
    "x + y \\leq x - y \\\\\n",
    "y \\leq -y \n",
    "\\end{gathered}\n",
    "\n",
    "For $x + y < 0$:\n",
    "\\begin{gathered}\n",
    "-(x + y) \\leq x - y \\\\\n",
    "-x - y \\leq x - y \\\\\n",
    "-x \\leq x \n",
    "\\end{gathered}\n",
    "\n",
    "$ \\textbf{Case 4:} $ $x < 0, y \\geq 0$\n",
    "\n",
    "- Let, $|x| = -x, |y| = y$\n",
    "- Substitution:\n",
    "\\begin{gathered}\n",
    "|x + y| \\leq -x + y\n",
    "\\end{gathered}\n",
    "- Solve for sub-cases of $|x + y|$:\n",
    "\\begin{gathered}\n",
    "x + y, x + y \\geq 0 \\\\\n",
    "-(x + y), x + y < 0 \\\\\n",
    "\\end{gathered}\n",
    "\n",
    "For $x + y \\geq 0$:\n",
    "\\begin{gathered}\n",
    "x + y \\leq -x + y \\\\\n",
    "x \\leq -x\n",
    "\\end{gathered}\n",
    "\n",
    "For $x + y < 0$:\n",
    "\\begin{gathered}\n",
    "-(x + y) \\leq -x + y \\\\\n",
    "-x - y \\leq -x + y \\\\\n",
    "-y \\leq y\n",
    "\\end{gathered}\n",
    "\n",
    "<br><br>\n",
    "\n",
    "<br>\n",
    "\n",
    "**In conclusion from  all the cases we have shown, this proves the triangle inequality for all real numbers $x$ and $y$.**\n",
    "\n",
    "\n",
    "****\n"
   ]
  },
  {
   "cell_type": "markdown",
   "metadata": {},
   "source": [
    "### $\\textbf{Problem 4:}$\n",
    "\n",
    "<b><u>Problem</u></b>\n",
    "\n",
    "Prove Sedrakayan's Lemma $\\forall u_i, v_i \\in \\mathbb{R}^+$:\n",
    "\\begin{gather}\n",
    "\\frac{(\\Sigma_{i=1}^n u_i)^2}{\\Sigma_{i=1}^n v_i}\n",
    "\\leq\n",
    "\\Sigma_{i=1}^n \\frac{(u_i)^2}{v_i}\n",
    "\\end{gather}\n",
    "\n",
    "<b><u>Solution</u></b>\n",
    "\n",
    "<b> Step 1: </b> \n",
    "\n",
    "Since we want are going prove Sedrakayan's Lemma, Which states that: \n",
    "\n",
    "- For any positive real numbers $u_i$ and $v_i$ (where $i$ ranges from 1 to $n$):\n",
    "\\begin{gathered} \\frac{\\left(\\sum_{i=1}^n u_i\\right)^2}{\\sum_{i=1}^n v_i} \\leq \\sum_{i=1}^n \\frac{u_i^2}{v_i} \\end{gathered}\n",
    "\n",
    "\n",
    "So to prove this, we'll be using the cauchy-Schwarz Inequality \n",
    "\n",
    "<b>Step 2: </b> \n",
    "\n",
    "Define the equations\n",
    "- $\\mathbf{u} = (u_1, u_2, ..., u_n)$\n",
    "- $\\mathbf{v} = (\\sqrt{v_1}, \\sqrt{v_2}, ..., \\sqrt{v_n})$\n",
    "\n",
    "\n",
    "<b>Step 3: </b> \n",
    "\n",
    "Once that's done, we apply the Cauchy-Schwarz Inequality for inner products of vectors. This inequality states that the square of the dot product of two vectors is less than or equal to the product of the squares of their magnitudes.\n",
    "\n",
    "For the sum of $u_i$, we have:\n",
    "- $\\left(\\sum_{i=1}^n u_i\\right)^2 \\leq n \\left(\\sum_{i=1}^n u_i^2\\right)$\n",
    "\n",
    "For the sum of $\\sqrt{v_i}$, we have:\n",
    "- $\\left(\\sum_{i=1}^n \\sqrt{v_i}\\right)^2 \\leq n \\left(\\sum_{i=1}^n v_i\\right)$\n",
    "\n",
    "<b>Step 4: </b> \n",
    "\n",
    "Next, we have to rearrange the equation. Once we've done that we get:\n",
    "- $\\frac{\\left(\\sum_{i=1}^n u_i\\right)^2}{\\sum_{i=1}^n v_i} \\leq \\frac{\\sum_{i=1}^n u_i^2}{\\sum_{i=1}^n v_i}$\n",
    "\n",
    "<b>Step 5: </b> \n",
    "\n",
    "Finally, once we've deduced that, this will be our final answer.\n",
    "\\begin{gathered} \\frac{\\left(\\sum_{i=1}^n u_i\\right)^2}{\\sum_{i=1}^n v_i} \\leq \\frac{\\sum_{i=1}^n u_i^2}{\\sum_{i=1}^n v_i} \\end{gathered}\n",
    "\n",
    "\n",
    "**Therefore we conclude, that we have proven Sedrakayan's Lemma.**"
   ]
  }
 ],
 "metadata": {
  "language_info": {
   "name": "python"
  }
 },
 "nbformat": 4,
 "nbformat_minor": 2
}
